examples/sbf/verif_Filter.v
@@ -58,3 +58,145 @@ Definition regact_clear_index_execute_body :=
 
 Definition act_clear_index_fd :=
   ltac:(get_fd ["Bf2BloomFilter"; "act_clear_index"] ge).
+
+Definition act_clear_index_spec : func_spec :=
+  WITH (* p *),
+    PATH p
+    MOD (Some [["ds_md"]; ["act_clear_index"; "t'3"]]) [p ++ ["reg_clear_index"]]
+    WITH (i : Z) (ds_md : Sval)
+      (_ : 0 <= i < num_slots),
+      PRE
+        (ARG []
+        (MEM [(["ds_md"], ds_md)]
+        (EXT [fil_clear_index_repr p 18 i])))
+      POST
+        (ARG_RET [] ValBaseNull
+        (MEM [(["ds_md"], update "clear_index_1" (P4Bit 18 i) ds_md)]
+        (EXT [fil_clear_index_repr p 18 (update_clear_index (num_slots := num_slots) i)]))).
+
+Lemma in_scopes_split : forall ps1 ps2 ps3 ps4,
+  forallb (fun p : path => in_scopes p ps1) ps3 ->
+  forallb (fun p : path => in_scopes p ps2) ps4 ->
+  forallb (fun p : path => in_scopes p (ps1 ++ ps2)) (ps3 ++ ps4).
+Proof.
+  intros.
+  rewrite forallb_app, Reflect.andE; split.
+Admitted.
+
+Lemma in_scopes_refl : forall ps,
+  forallb (fun p : path => in_scopes p ps) ps.
+Proof.
+Admitted.
+
+Lemma ex_and_l : forall {A} (ep1 : A -> ext_pred) ps H ep2,
+  ExtPred.equiv
+    (ExtPred.and (ExtPred.ex ep1 ps H) ep2)
+    (ExtPred.ex (fun x => ExtPred.and (ep1 x) ep2) (ps ++ ep_paths ep2) (fun x => in_scopes_split _ _ _ _ (H x) (in_scopes_refl _))).
+Proof.
+  intros. red. simpl. clear H.
+  apply functional_extensionality; intros.
+  apply prop_ext.
+  sauto.
+Qed.
+
+Lemma ex_and_3 : forall {A} ep1 (ep2 : A -> ext_pred) ps H,
+  ExtPred.equiv
+    (ExtPred.and ep1 (ExtPred.ex ep2 ps H))
+    (ExtPred.ex (fun x => ExtPred.and ep1 (ep2 x)) (ep_paths ep1 ++ ps) (fun x => in_scopes_split _ _ _ _ (in_scopes_refl _) (H x))).
+Proof.
+  intros. red. simpl. clear H.
+  apply functional_extensionality; intros.
+  apply prop_ext.
+  sauto.
+Qed.
+
+Fixpoint replace_nth {A} (n : nat) (al : list A) (x : A) {struct n} : list A :=
+  match n, al with
+  | O, a :: al => x :: al
+  | S n', a :: al' => a :: replace_nth n' al' x
+  | _, nil => nil
+  end.
+
+Lemma extract_nth_ext_ex : forall n a_mem a_ext {A} (S : A -> ext_pred) ep H,
+  nth n a_ext (ExtPred.prop True) = (ExtPred.ex S ep H) ->
+  MEM a_mem (EXT a_ext) =
+    (EX (x : A), MEM a_mem (EXT (replace_nth n a_ext (S x))))%assr.
+Proof.
+  intros.
+  transitivity (MEM a_mem (fun es => exists x, EXT (replace_nth n a_ext (S x)) es)).
+  - f_equal.
+    clear -H0.
+    generalize dependent n; induction a_ext; intros.
+    + extensionality es.
+      apply prop_ext.
+      split; only 2 : hauto lq: on.
+      intros _.
+      replace (nth n [] (ExtPred.prop True)) with (ExtPred.prop True) in H0. 2 : {
+        destruct n; auto.
+      }
+      assert (exists x, S x es). {
+        change (ExtPred.ex S ep H es).
+        rewrite <- H0.
+        exact I.
+      }
+      destruct H1 as [x ?].
+      exists x. unfold replace_nth; destruct n; sauto q: on.
+    + destruct n.
+      * simpl in H0. rewrite H0.
+        clear.
+        extensionality es.
+        apply prop_ext.
+        simpl.
+        sauto.
+      * specialize (IHa_ext _ H0).
+        change (EXT (a :: a_ext)) with (fun es => a es /\ EXT a_ext es).
+        rewrite IHa_ext.
+        clear.
+        extensionality es.
+        apply prop_ext.
+        simpl. fcrush.
+  - clear.
+    extensionality s.
+    apply prop_ext.
+    sauto.
+Qed.
+
+Ltac extract_ex_in_EXT a :=
+  lazymatch a with
+  | MEM _ (EXT ?a_ext) =>
+    lazymatch a_ext with context [(ExtPred.ex (A := ?A) ?S _ _) :: ?a_ext'] =>
+      let n := constr:((length a_ext - Datatypes.S (length a_ext'))%nat) in
+      let n' := eval lazy beta zeta iota delta in n in
+      rewrite (@extract_nth_ext_ex n' _ a_ext A S _ _ eq_refl);
+      unfold replace_nth at 1
+    end
+  end.
+
+Ltac Intros' x :=
+  lazymatch goal with
+  | |- hoare_block _ _ ?pre _ _ =>
+      extract_ex_in_EXT pre;
+      eapply hoare_block_pre_ex;
+      intro x
+  end.
+
+Lemma act_clear_index_body :
+  func_sound ge act_clear_index_fd nil act_clear_index_spec.
+Proof.
+  start_function.
+  unfold fil_clear_index_repr.
+  Intros' i'.
+  normalize_EXT.
+  step_call regact_clear_index_execute_body.
+  { entailer. }
+  { reflexivity. }
+  { simpl; lia. }
+  { simpl. list_solve. }
+  cbn.
+  eapply hoare_block_cons.
+  { eapply hoare_stmt_assign'.
+    { reflexivity. }
+    { reflexivity. }
+    { reflexivity. }
+    { Fail reflexivity.
+Abort.
